\documentclass[varwidth=1000pt]{standalone}
\usepackage{ebproof}
\begin{document}
(not (<= (+ (f (x1 ) (0 )) (* (- (1 )) (x3 ))) (- (1 ))))

Proof/Definition of a!1

(not (>= (+ (f (x1 ) (0 )) (* (- (1 )) (x3 ))) (0 )))

Proof/Definition of a!2

(= (>= (f (x1 ) (0 )) (x3 )) (>= (+ (f (x1 ) (0 )) (* (- (1 )) (x3 ))) (0 )))

Proof/Definition of a!3

\begin{prooftree}\infer0[definition]{else}   \infer1[asserted]{something}\end{prooftree}

Proof/Definition of a!5

(= (- (x3 ) (f (x1 ) (0 ))) (+ (x3 ) (* (- (1 )) (f (x1 ) (0 )))))

Proof/Definition of a!6

(>= (+ (x3 ) (* (- (1 )) (f (x1 ) (0 )))) (1 ))

Proof/Definition of a!7

(= (+ (x3 ) (* (- (1 )) (f (x1 ) (0 )))) (+ (* (- (1 )) (f (x1 ) (0 ))) (x3 )))

Proof/Definition of a!9

(>= (+ (* (- (1 )) (f (x1 ) (0 ))) (x3 )) (1 ))

Proof/Definition of a!10

\begin{prooftree}\infer0[definition]{else}  \infer1[asserted]{something} \infer0[definition]{else}\infer1[rewrite]{something} \infer0[definition]{else}    \infer3[mp]{something}\end{prooftree}

Proof/Definition of a!4

(= (>= (- (x3 ) (f (x1 ) (0 ))) (1 )) (a!7 ))

Proof/Definition of a!8

(= (a!10 ) (<= (+ (f (x1 ) (0 )) (* (- (1 )) (x3 ))) (- (1 ))))

Proof/Definition of a!11

(= (a!7 ) (<= (+ (f (x1 ) (0 )) (* (- (1 )) (x3 ))) (- (1 ))))

Proof/Definition of a!12

\begin{prooftree}\infer0[definition]{else} \infer0[definition]{else}\infer1[rewrite]{something} \infer0[definition]{else}\infer2[monotonicity]{something} \infer0[definition]{else}\infer3[mp]{something} \infer0[definition]{else}\infer1[rewrite]{something} \infer0[definition]{else} \infer2[monotonicity]{something} \infer0[definition]{else}\infer1[rewrite]{something} \infer0[definition]{else}\infer3[trans]{something} \infer0[definition]{else}    \infer3[mp]{something}\end{prooftree}

Proof/Definition of a!13

\begin{prooftree}\infer0[definition]{else} \infer1[th-lemma]{something} \infer0[definition]{else} \infer0[definition]{else} \infer0[definition]{else}\infer4[unit-resolution]{something}\end{prooftree}
\end{document}

