\documentclass{article}
\begin{document}





















































































































































































































































$(\exists (x_{0} : Int). \\(\forall (x_{1} : Array(Int, Int)). \\(\exists (x_{2} : Array(Int, Int)). \\(\forall (x_{3} : Int). \\(\exists (x_{4} : Int), (x_{5} : Int). \\(\forall (x_{6} : Int). \\(\exists (x_{7} : Array(Int, Int)). \\(\forall (x_{8} : Array(Int, Int)). \\(\exists (x_{9} : Int), (x_{10} : Array(Int, Int)). \\(\forall (x_{11} : Int), (x_{12} : Int), (x_{13} : Int), (x_{14} : Int). \\(\exists (x_{15} : Int). \\(\forall (x_{16} : Int). \\let \\a!1 = (x_{9} = select( store(x_{10}, x_{6}, x_{11}), array-ext(x_{7}, x_{8})))\\ a!3 = ((\neg (array-ext(x_{2}, x_{1}) = x_{16})) \lor (\neg (select( array_{t_{4}}, x_{16}) = x_{3})))\\ a!4 = ((x_{15} = array-ext(x_{2}, x_{1})) \land (\neg (select( array_{s_{4}}, x_{15}) = x_{3})) \land q_{3}(x_{15}) \land q_{2}(x_{15}) \land q_{1}(x_{15}) \land p_{4}(x_{15}))\\ a!5 = ((x_{0} = array-ext(x_{2}, x_{1})) \land (\neg (select( array_{s_{2}}, x_{0}) = x_{3})) \land p_{2}(x_{0}) \land q_{1}(x_{0}))\\ a!6 = ((x_{4} = array-ext(x_{2}, x_{1})) \land (\neg (select( array_{s_{3}}, x_{4}) = x_{3})) \land q_{1}(x_{4}) \land p_{3}(x_{4}) \land q_{2}(x_{4}))\\ a!7 = ((x_{5} = array-ext(x_{2}, x_{1})) \land (\neg (select( array_{s_{1}}, x_{5}) = x_{3})) \land p_{1}(x_{5}))\\ a!8 = (\neg ((array-ext(x_{7}, x_{8}) = x_{14}) \land (x_{1} = x_{8})))\\ a!13 = ((\neg (array-ext(x_{2}, x_{1}) = x_{12})) \lor (\neg (select( array_{t_{2}}, x_{12}) = x_{3})) \lor p_{1}(x_{12}) \lor q_{2}(x_{12}) \lor p(x_{1}))\\ a!14 = ((\neg (array-ext(x_{2}, x_{1}) = x_{13})) \lor (\neg (select( array_{t_{3}}, x_{13}) = x_{3})) \lor p_{2}(x_{13}) \lor q_{3}(x_{13}) \lor p_{1}(x_{13}) \lor p(x_{1}))\\ a!16 = ((\neg (array-ext(x_{2}, x_{1}) = x_{16})) \lor (\neg (select( array_{s_{2}}, x_{0}) = x_{3}))) in \\let \\a!2 = (a!1 \land (select( store(s, x_{6}, x_{11}), array-ext(x_{2}, x_{8})) = x_{3}))\\ a!9 = (a!8 \lor (\neg (select( array_{t_{1}}, x_{14}) = x_{3})))\\ a!10 = (a!8 \lor (\neg (select( array_{s_{2}}, x_{0}) = x_{3})))\\ a!11 = (a!8 \lor (\neg (select( array_{s_{4}}, x_{15}) = x_{3}))) in \\let \\a!12 = (((array-ext(x_{7}, x_{8}) = array-ext(x_{2}, x_{8})) \land a!9) \lor q_{1}(x_{14}) \lor ((x_{0} = x_{14}) \land (array-ext(x_{7}, x_{8}) = array-ext(x_{2}, x_{8})) \land a!10 \land p_{2}(x_{0}) \land q_{1}(x_{0})) \lor p(x_{1}) \lor ((x_{15} = x_{14}) \land (array-ext(x_{7}, x_{8}) = array-ext(x_{2}, x_{8})) \land a!11 \land q_{3}(x_{15}) \land q_{2}(x_{15}) \land q_{1}(x_{15}) \land p_{4}(x_{15})))\\ a!17 = ((\neg a!2) \land (((x_{0} = x_{16}) \land a!16 \land p_{2}(x_{0}) \land q_{1}(x_{0})) \lor p(x_{1}))) in \\let \\a!15 = ((((\neg a!2) \land a!3) \lor a!4 \lor p(x_{1}) \lor a!5 \lor a!6 \lor a!7) \land a!12 \land ((x_{6} = array-ext(x_{7}, x_{8})) \lor a!1) \land a!13 \land a!14)\\ a!18 = ((a!17 \lor a!4 \lor p(x_{1}) \lor a!5 \lor a!6 \lor a!7) \land a!12 \land ((x_{6} = array-ext(x_{7}, x_{8})) \lor a!1) \land a!13 \land a!14) in \\let \\a!19 = (((\neg a!2) \land (a!15 \lor p(x_{1}) \lor q_{4}(x_{16}) \lor p_{1}(x_{16}) \lor a!18 \lor p_{3}(x_{16}))) \lor a!4 \lor p(x_{1}) \lor a!5 \lor a!6 \lor a!7) in \\let \\a!20 = (a!19 \land a!12 \land ((x_{6} = array-ext(x_{7}, x_{8})) \lor a!1) \land a!13 \land a!14) in \\(a!20 \lor p(x_{1}))))))))))))))$

\end{document}


